# Lagrangian
$$
T = \frac{1}{2}m_1(l_1\dot{\theta}_1)^2 + \frac{1}{2}\frac{1}{12}m_1l_1^2\dot{\theta}_1^2+\frac{1}{2}m_2(\frac{l_2\dot{\theta}_2}{2}+l_1\dot{\theta}_1)^2 + \frac{1}{2}\frac{1}{12}m_2l_2^2\dot{\theta}_2^2
$$

$$
V = -gm_1\frac{l_1}{2}\cos{\theta_1}-gm_2(l_1\cos{\theta_1}+\frac{l_2}{2}\cos{\theta_2})
$$

$$
L = T-V
$$

$$
(\frac{1}{3}m_1l_1^2+m_2l_2^2)\ddot{\theta}_1+(\frac{1}{2}m_2l_1l_2)\ddot{\theta}_2=-(\frac{m_1}{2}+m_2)gl_1\sin{\theta}_1
$$

$$
(\frac{1}{2}m_2l_1l_2)\ddot{\theta}_1+(\frac{1}{3}m_2l_2^2)\ddot{\theta}_2=-(\frac{m_2}{2})gl_2\sin{\theta_2}
$$

$$
\ddot{\theta}_1=-\frac{3(gl_1m_1\sin{\theta_1}+2gl_1m_2\sin{\theta_1}-gl_2m_2\sin{\theta_2})}{2l_1^2m_1-3l_1l_2m_2+6l_2^2m_2}
$$

$$
\ddot{\theta}_2=-\frac{3(-3gl_1^2m_1\sin{\theta_1}-6gl_1^2m_2\sin{\theta_1}+2gl_1^2m_1\sin{\theta_2}+6gl_2^2m_2\sin{\theta_2})}{2l_2(2l_1^2m_1-3l_1l_2m_2+6l_2^2m_2)}
$$